theories/Compositional_Structures/Basic_Modules/Component_Types/Elimination_Module_Ref.thy
@@ -56,9 +56,6 @@ definition eliminate:: "'a Scores_Map  \<Rightarrow> Threshold_Value \<Rightarro
     }) ({}, {})
 }"
 
-(* Needed for Sepref Correctness Proof When uncurrying Alternatives and Profile  *)
-type_synonym 'a Electoral_Module_Ref_Cur = "('a set \<times> 'a Profile_List) \<Rightarrow> 'a Result nres"
-
 
 definition elimination_module_ref :: 
 "'a Scores_Map  \<Rightarrow> Threshold_Value \<Rightarrow>
@@ -85,13 +82,13 @@ lemma eliminate_correct:
   and r :: "Threshold_Relation"
   shows "((\<lambda> A. eliminate (pre_computed_map e A p) t r A), 
     (\<lambda> A. SPEC (\<lambda> (rej,def). (rej,def) = ((elimination_set e t r A p), A - (elimination_set e t r A p)))))
-    \<in> \<langle>Id\<rangle>alt_set_rel \<rightarrow> \<langle>Id\<rangle>nres_rel"
+    \<in> \<langle>Id\<rangle>finite_set_rel \<rightarrow> \<langle>Id\<rangle>nres_rel"
   unfolding pre_computed_map_def eliminate_def
 proof (refine_vcg, rename_tac A' A)
   fix A' A :: "'a set"
-  assume arel: "(A', A) \<in> \<langle>Id\<rangle>alt_set_rel"
-  from arel have aeq: "A' = A" by (auto simp add: alt_set_rel_def in_br_conv)
-  from arel have fina: "finite A'" by (auto simp add: alt_set_rel_def in_br_conv)
+  assume arel: "(A', A) \<in> \<langle>Id\<rangle>finite_set_rel"
+  from arel have aeq: "A' = A" by (auto simp add: finite_set_rel_def in_br_conv)
+  from arel have fina: "finite A'" by (auto simp add: finite_set_rel_def in_br_conv)
   show " FOREACH A'
         (\<lambda>x (rej, def).
             ASSERT (x \<in> dom ((\<lambda>a. Some (e a A' p)) |` A')) \<bind>
@@ -109,7 +106,7 @@ qed
 
 lemma compute_scores_correct:
   shows "(pre_compute_scores, (\<lambda> e A pr. SPEC(\<lambda> map. map = (pre_computed_map e A pr)))) \<in> 
-   evalf_rel \<rightarrow> \<langle>Id\<rangle>alt_set_rel \<rightarrow> profile_rel \<rightarrow> \<langle>Id\<rangle>nres_rel"
+   evalf_rel \<rightarrow> \<langle>Id\<rangle>finite_set_rel \<rightarrow> profile_rel \<rightarrow> \<langle>Id\<rangle>nres_rel"
   unfolding pre_compute_scores_def pre_computed_map_def
 proof (refine_vcg, rename_tac eref efun A' A pl pr )
   fix eref :: "'a Evaluation_Function_Ref" 
@@ -118,10 +115,10 @@ proof (refine_vcg, rename_tac eref efun A' A pl pr )
   fix pl :: "'a Profile_List"
   fix pr :: "'a Profile"
   assume eref_refine: "(eref, efun) \<in> evalf_rel"
-  assume arel: "(A', A) \<in> \<langle>Id\<rangle>alt_set_rel"
+  assume arel: "(A', A) \<in> \<langle>Id\<rangle>finite_set_rel"
   assume profrel: " (pl, pr) \<in> profile_rel"
-  from arel have aeq: "A' = A" by (auto simp add: alt_set_rel_def in_br_conv)
-  from arel have fina: "finite A'" by (auto simp add: alt_set_rel_def in_br_conv)
+  from arel have aeq: "A' = A" by (auto simp add: finite_set_rel_def in_br_conv)
+  from arel have fina: "finite A'" by (auto simp add: finite_set_rel_def in_br_conv)
   show "       FOREACH A' (\<lambda>x m. eref x A' pl \<bind> (\<lambda>scx. RETURN (m(x \<mapsto> scx)))) Map.empty
        \<le> SPEC (\<lambda>map. map = (\<lambda>a. Some (efun a A pr)) |` A)"
   proof (refine_vcg FOREACH_rule[where I = 
@@ -166,13 +163,12 @@ proof (clarify, refine_vcg, rename_tac e e_ref A' pl A pr )
   fix pr :: "'a Profile"
   fix a:: 'a
   assume rel: "((A', pl), A, pr) \<in> \<langle>Id\<rangle>alt_and_profile_rel"
-  from rel have arel : "(A', A) \<in> \<langle>Id\<rangle>alt_set_rel" 
+  from rel have arel : "(A', A) \<in> \<langle>Id\<rangle>finite_set_rel" 
     using unfold_alt_profile_alt_rel by blast
   from rel have prel: "(pl, pr) \<in> profile_rel " using unfold_alt_profile_prof_rel
     by blast
-  from arel have aeq: "A' = A" by (auto simp add: alt_set_rel_def in_br_conv)
-  from arel have fina: "finite A" by (auto simp add: alt_set_rel_def in_br_conv)
-  from arel have nempa: "A \<noteq> {}" by (auto simp add: alt_set_rel_def in_br_conv)
+  from arel have aeq: "A' = A" by (auto simp add: finite_set_rel_def in_br_conv)
+  from arel have fina: "finite A" by (auto simp add: finite_set_rel_def in_br_conv)
   assume eref_refine: "(eref, efun) \<in> evalf_rel_prof"
   from rel have profprop: "profile_l A pl" using aeq unfold_alt_profile_prof_prop
     by blast
@@ -218,19 +214,20 @@ theorem elimination_module_ref_correct:
   assumes "(pl, pr) \<in> profile_rel"
 shows "(\<lambda> A. (elimination_module_ref (pre_computed_map efn A pr) t r A pl),
         (\<lambda> A. SPEC (\<lambda> em. em = (elimination_module efn t r A pr))))
-      \<in> \<langle>Id\<rangle>alt_set_rel \<rightarrow> \<langle>\<langle>Id\<rangle>set_rel \<times>\<^sub>r \<langle>Id\<rangle>set_rel \<times>\<^sub>r \<langle>Id\<rangle>set_rel\<rangle>nres_rel"
+      \<in> \<langle>Id\<rangle>finite_set_rel \<rightarrow> \<langle>\<langle>Id\<rangle>set_rel \<times>\<^sub>r \<langle>Id\<rangle>set_rel \<times>\<^sub>r \<langle>Id\<rangle>set_rel\<rangle>nres_rel"
   unfolding em_rel_def
   unfolding elimination_module_ref_def
 proof (clarify, rename_tac A' A)
   fix A' A :: "'a set"
-  assume arel: "(A', A) \<in> \<langle>Id\<rangle>alt_set_rel"
+  assume arel : "(A', A) \<in> \<langle>Id\<rangle>finite_set_rel"
   note elimalg = eliminate_correct[THEN fun_relD, THEN nres_relD, THEN refine_IdD,
           where x2=A' and x'2 = A]
-  from arel have " (eliminate (pre_computed_map efn A' pr) t r A' \<bind>
+   have " (eliminate (pre_computed_map efn A' pr) t r A' \<bind>
         (\<lambda>(rej, def). if def = {} then RETURN ({}, {}, rej) else RETURN ({}, rej, def)),
         SPEC (\<lambda>em. em = elimination_module efn t r A pr))
        \<in> \<langle>Id\<rangle>nres_rel"
-    by (refine_vcg elimalg, auto)
+     apply (refine_vcg elimalg)
+     by (auto simp add: arel)
   from this show "(eliminate (pre_computed_map efn A' pr) t r A' \<bind>
         (\<lambda>(rej, def). if def = {} then RETURN ({}, {}, rej) else RETURN ({}, rej, def)),
         SPEC (\<lambda>em. em = elimination_module efn t r A pr))
@@ -239,48 +236,42 @@ proof (clarify, rename_tac A' A)
 qed
 
 lemma scoremax_correct:
+  fixes A :: "'a set"
+  assumes fina: "finite A" and nempa: "A \<noteq> {}"
   fixes e :: "'a Evaluation_Function"
   and pr :: "'a Profile"
-  shows "((\<lambda> A. scoremax A (pre_computed_map e A pr)),
- (\<lambda> A.  SPEC (\<lambda> max. max = Max {(e a A pr) | a. a \<in> A})))
-  \<in> \<langle>Id\<rangle>alt_set_rel \<rightarrow> \<langle>Id\<rangle>nres_rel"
-  unfolding scoremax_def pre_computed_map_def
-proof (clarify, rename_tac A' A)
-  fix A' A :: "'a set"
-  assume arel: "(A', A) \<in> \<langle>Id\<rangle>alt_set_rel"
-  from arel have aeq: "A' = A" by (auto simp add: alt_set_rel_def in_br_conv)
-  from arel have fina: "finite A" by (auto simp add: alt_set_rel_def in_br_conv)
-  from arel have nempa: " A \<noteq> {}" by (auto simp add: alt_set_rel_def in_br_conv)
-  show "(FOREACH A'
-         (\<lambda>x max.
-             ASSERT (x \<in> dom ((\<lambda>a. Some (e a A' pr)) |` A')) \<bind>
-             (\<lambda>_. let scx = the (((\<lambda>a. Some (e a A' pr)) |` A') x)
-                   in if max < scx then RETURN scx else RETURN max))
-         0,
-        SPEC (\<lambda>max. max = Max {e a A pr |a. a \<in> A}))
-       \<in> \<langle>nat_rel\<rangle>nres_rel"
-  apply (refine_vcg FOREACH_rule[where I = "(\<lambda>it max. (\<forall>a \<in> (A - it). (e a A pr) \<le> max)
-      \<and> ((\<exists>a \<in> (A - it). max = (e a A pr)) \<or> max = 0))"], clarsimp_all simp add: aeq fina nempa,
+  shows "scoremax A (pre_computed_map e A pr)
+ \<le> SPEC (\<lambda> max. max = Max {(e a A pr) | a. a \<in> A})"
+proof (unfold scoremax_def pre_computed_map_def)
+  show "FOREACH A
+     (\<lambda>x max.
+         ASSERT (x \<in> dom ((\<lambda>a. Some (e a A pr)) |` A)) \<bind>
+         (\<lambda>_. let scx = the (((\<lambda>a. Some (e a A pr)) |` A) x)
+               in if max < scx then RETURN scx else RETURN max))
+     0
+    \<le> SPEC (\<lambda>max. max = Max {e a A pr |a. a \<in> A})"
+    apply (refine_vcg FOREACH_rule[where I = "(\<lambda>it max. (\<forall>a \<in> (A - it). (e a A pr) \<le> max)
+      \<and> ((\<exists>a \<in> (A - it). max = (e a A pr)) \<or> max = 0))"], clarsimp_all simp add:  fina nempa,
          auto)
   using max_score_in[where A= A and f = "(\<lambda> x. e x A pr)"] fina nempa
-            score_bounded[where A= A and f = "(\<lambda> x. e x A pr)"] aeq
+            score_bounded[where A= A and f = "(\<lambda> x. e x A pr)"] 
   apply (metis DiffI dual_order.trans order_less_imp_le)
   using max_score_in[where A= A and f = "(\<lambda> x. e x A pr)"] fina nempa
-            score_bounded[where A= A and f = "(\<lambda> x. e x A pr)"] aeq
-  subgoal by (metis (mono_tags, lifting) order_antisym_conv)
-proof -
-  assume "\<forall>a\<in>A. e a A pr = 0"
-  from this have eq: "{e a A pr |a. a \<in> A} = {0}"
+            score_bounded[where A= A and f = "(\<lambda> x. e x A pr)"] 
+proof ((metis (mono_tags, lifting) order_antisym_conv))
+  assume all0: "\<forall>a\<in>A. e a A pr = 0"
+  from all0 have eq: "{e a A pr |a. a \<in> A} = {0}"
     using nempa Max_singleton by force
   have "Max {0} = 0"
     using Max_singleton by blast
-  from eq this show " Max {e a A pr |a. a \<in> A} = 0"
+  from eq this  show " Max {e a A pr |a. a \<in> A} = 0"
     by simp
 qed
 qed
 
-context set_of_alternatives
+(*context set_of_alternatives
 begin
+
 
 
 lemma scoremax_correct_ctx:
@@ -306,7 +297,7 @@ proof -
     by simp
 qed
 
-end
+end*)
  
 
 locale profile_complete = set_of_alternatives + 
@@ -314,55 +305,21 @@ locale profile_complete = set_of_alternatives +
   assumes 
      profrel: "(pl, pr) \<in> profile_on_A_rel A"
 
-context profile_complete
-begin
-
-lemma compute_scores_correct_weak_evalref:
-  fixes eref :: "'a Evaluation_Function_Ref"
-  and e :: "'a Evaluation_Function"
-  assumes "((\<lambda> x. eref x A), (\<lambda> x p. RETURN ( e x A p))) \<in> evalf_profA_rel A"
-  shows "(pre_compute_scores eref A pl, SPEC (\<lambda> map. map = pre_computed_map e A pr)) \<in> 
-    \<langle>Id\<rangle>nres_rel"
-  unfolding pre_compute_scores_def pre_computed_map_def
-  apply (refine_vcg FOREACH_rule[where I = 
-        "(\<lambda> it r. r = (\<lambda> a. Some (e a A pr))|`(A - it))"])
-  apply (auto simp add: fina)
-proof -
-  fix x:: 'a
-  fix it:: "'a set"
-  assume xit: "x \<in> it"
-  assume itA: "it \<subseteq> A"
-  from xit itA have xiA: "x \<in> A" by fastforce
-  from xit itA have wcr: "((\<lambda> a. Some (e a A pr)) |` (A - it))(x \<mapsto> (e x A pr)) =
-                      (\<lambda> a. Some (e a A pr)) |` (A - (it - {x}))"
-      using it_step_insert_iff restrict_map_insert
-      by metis
-  from this have mapupdeq: "(\<lambda> scx. ((\<lambda> a. Some (e a A pr)) |` (A - it))(x  \<mapsto> scx) =
-                   (\<lambda> a. Some (e a A pr)) |` (A - (it - {x})))
-      = (\<lambda> wc. wc = (e x A pr))"
-    by (metis map_upd_eqD1)
-  from profrel have prel: "(pl, pr) \<in> profile_rel" using profile_type_ref by auto
-  from profrel assms(1)[THEN fun_relD, THEN fun_relD, THEN nres_relD]
-    this have "(eref x A pl) \<le> SPEC(\<lambda> scx. scx = (e x A pr))"
-    by (metis IdI SPEC_eq_is_RETURN(2) refine_IdD) 
-  from this mapupdeq show " (eref x A pl)
-       \<le> SPEC (\<lambda> scx. ((\<lambda> a. Some (e a A pr)) |` (A - it))(x \<mapsto> scx) =
-                      (\<lambda> a. Some (e a A pr)) |` (A - (it - {x})))"
-    using SPEC_cons_rule it_step_insert_iff restrict_map_insert
-    by presburger 
-qed 
-end
 
 
 subsection \<open>Common Eliminators\<close>
                                    
-fun less_eliminator_ref :: "'a Scores_Map  \<Rightarrow> Threshold_Value \<Rightarrow>
+definition less_eliminator_ref :: "'a Scores_Map  \<Rightarrow> Threshold_Value \<Rightarrow>
                             'a Electoral_Module_Ref" where
-  "less_eliminator_ref e t A p = elimination_module_ref e t (<) A p"
+  "less_eliminator_ref e t A p \<equiv> elimination_module_ref e t (<) A p"
 
-fun max_eliminator_ref ::  "'a Scores_Map \<Rightarrow>
+definition max_eliminator_ref ::  "'a Scores_Map \<Rightarrow>
                             'a Electoral_Module_Ref" where
-  "max_eliminator_ref e A p = do {
+  "max_eliminator_ref e A p \<equiv>
+    if (A = {}) then
+      RETURN ({},{},{})
+    else do {
+    ASSERT (A \<noteq> {});
     t <- (scoremax A e); 
     (less_eliminator_ref e t A p)
  }"
@@ -375,11 +332,11 @@ lemma less_eliminator_correct:
   assumes prel: "(pl, pr) \<in> profile_rel"
   shows "((\<lambda> A. less_eliminator_ref (pre_computed_map efn A pr) t A pl),
             (\<lambda> A. SPEC (\<lambda> em. em = (less_eliminator efn t A pr))))
-          \<in> \<langle>Id\<rangle>alt_set_rel \<rightarrow> \<langle>\<langle>Id\<rangle>set_rel \<times>\<^sub>r \<langle>Id\<rangle>set_rel \<times>\<^sub>r \<langle>Id\<rangle>set_rel\<rangle>nres_rel"
-  unfolding less_eliminator_ref.simps less_eliminator.simps
+          \<in> \<langle>Id\<rangle>finite_set_rel \<rightarrow> \<langle>\<langle>Id\<rangle>set_rel \<times>\<^sub>r \<langle>Id\<rangle>set_rel \<times>\<^sub>r \<langle>Id\<rangle>set_rel\<rangle>nres_rel"
+  unfolding less_eliminator_ref_def less_eliminator.simps
 proof (clarify, rename_tac A' A)
   fix A' A :: "'a set"
-  assume arel: "(A', A) \<in> \<langle>Id\<rangle>alt_set_rel"
+  assume arel: "(A', A) \<in> \<langle>Id\<rangle>finite_set_rel"
   from arel prel show "(elimination_module_ref (pre_computed_map efn A' pr) t (<) A' pl,
         SPEC (\<lambda>em. em = elimination_module efn t (<) A pr))
        \<in> \<langle>\<langle>Id\<rangle>set_rel \<times>\<^sub>r \<langle>Id\<rangle>set_rel \<times>\<^sub>r \<langle>Id\<rangle>set_rel\<rangle>nres_rel"
@@ -391,34 +348,46 @@ theorem max_eliminator_ref_correct:
   and pr :: "'a Profile"
   and pl :: "'a Profile_List"
   assumes prel: "(pl, pr) \<in> profile_rel"
-  shows "((\<lambda> A. max_eliminator_ref (pre_computed_map efn A pr) A pl),
+  shows "((\<lambda> A'. max_eliminator_ref (pre_computed_map efn A' pr) A' pl),
            ((\<lambda> A.  SPEC (\<lambda> em. em = max_eliminator efn A pr))))
- \<in> \<langle>Id\<rangle>alt_set_rel \<rightarrow>  \<langle>\<langle>Id\<rangle>set_rel \<times>\<^sub>r \<langle>Id\<rangle>set_rel \<times>\<^sub>r \<langle>Id\<rangle>set_rel\<rangle>nres_rel"
-  unfolding max_eliminator_ref.simps max_eliminator.simps
-proof (clarify, rename_tac A' A)
+ \<in> \<langle>Id\<rangle>finite_set_rel \<rightarrow>  \<langle>\<langle>Id\<rangle>set_rel \<times>\<^sub>r \<langle>Id\<rangle>set_rel \<times>\<^sub>r \<langle>Id\<rangle>set_rel\<rangle>nres_rel"
+  unfolding max_eliminator_ref_def 
+proof ( clarsimp simp del: max_eliminator.simps, rename_tac A' A, 
+    (refine_vcg))
   fix A' A :: "'a set"
-  assume arel: "(A', A) \<in> \<langle>Id\<rangle>alt_set_rel"
+  assume arel: "(A', A) \<in> \<langle>Id\<rangle>finite_set_rel"
+  assume empa: "A' = {}"
+  from arel have aeq: "A' = A" by (simp add: finite_set_rel_def in_br_conv)
+  from empa show "(({}, {}, {}), max_eliminator efn A pr) \<in> Id"
+    using aeq by auto  
+next
+  fix A' A :: "'a set"
+  assume arel: "(A', A) \<in> \<langle>Id\<rangle>finite_set_rel"
+  assume nempa: "A' \<noteq> {}"
+  from arel have fina: "finite A" by (simp add: finite_set_rel_def in_br_conv)
+  from arel have aeq: "A' = A" by (simp add: finite_set_rel_def in_br_conv)
+
   note lec = less_eliminator_correct[where efn = efn and t = "Max {efn x A pr |x. x \<in> A}",
-      THEN fun_relD, where x = A' and x' = A
-      and pl1 = pl and pr1 = pr, THEN nres_relD, THEN nres_relI]
-  from arel prel this have elim: "(less_eliminator_ref (pre_computed_map efn A' pr) (Max {efn x A pr |x. x \<in> A}) A' pl,
+      THEN fun_relD, THEN nres_relD, THEN nres_relI]
+  from arel prel this aeq have elim: "(less_eliminator_ref (pre_computed_map efn A' pr)
+   (Max {efn x A pr |x. x \<in> A}) A pl,
    SPEC (\<lambda>em. em = less_eliminator efn (Max {efn x A pr |x. x \<in> A}) A pr))
-  \<in> \<langle>\<langle>Id\<rangle>set_rel \<times>\<^sub>r \<langle>Id\<rangle>set_rel \<times>\<^sub>r \<langle>Id\<rangle>set_rel\<rangle>nres_rel" by simp
-  note sci = scoremax_correct[THEN fun_relD, THEN nres_relD, THEN refine_IdD]
-  from this arel prel have maxs: "scoremax A' (pre_computed_map efn A' pr) 
-    \<le> SPEC (\<lambda> maxs. maxs = (Max {efn x A pr |x. x \<in> A}))"
+  \<in> \<langle>\<langle>Id\<rangle>set_rel \<times>\<^sub>r \<langle>Id\<rangle>set_rel \<times>\<^sub>r \<langle>Id\<rangle>set_rel\<rangle>nres_rel"
+    by blast 
+  have simprefl: "less_eliminator_ref (pre_computed_map efn A' pr)
+   (Max {efn x A pr |x. x \<in> A}) A pl
+   \<le> SPEC (\<lambda>em. em = less_eliminator efn (Max {efn x A pr |x. x \<in> A}) A pr)"
+    using elim[THEN nres_relD]
+    by (clarsimp simp only: set_rel_id prod_rel_id refine_IdD)
+  note sci = scoremax_correct
+  from this arel prel fina nempa aeq have maxs: "scoremax A' (pre_computed_map efn A' pr) 
+    \<le> SPEC (\<lambda> maxs. maxs = (Max {efn x A pr |x. x \<in> A}))" 
     by blast
-  from elim maxs show "(scoremax A' (pre_computed_map efn A' pr) \<bind>
-        (\<lambda>t. less_eliminator_ref (pre_computed_map efn A' pr) t A' pl),
-        SPEC (\<lambda>em. em = less_eliminator efn (Max {efn x A pr |x. x \<in> A}) A pr))
-       \<in>  \<langle>\<langle>Id\<rangle>set_rel \<times>\<^sub>r \<langle>Id\<rangle>set_rel \<times>\<^sub>r \<langle>Id\<rangle>set_rel\<rangle>nres_rel"
-    using specify_left[where M = 
-        "\<Down> (\<langle>Id\<rangle>set_rel \<times>\<^sub>r \<langle>Id\<rangle>set_rel \<times>\<^sub>r \<langle>Id\<rangle>set_rel) 
-  (SPEC (\<lambda>em. em = less_eliminator efn (Max {efn x A pr |x. x \<in> A}) A pr))"
-        and m = "scoremax A' (pre_computed_map efn A' pr)"
-        and \<Phi> = "(\<lambda>maxs. maxs = Max {efn x A pr |x. x \<in> A})"
-        and f ="(\<lambda> x. less_eliminator_ref (pre_computed_map efn A' pr) x A' pl)"]
-  nres_relI nres_relD by blast
+  from simprefl maxs show " scoremax A' (pre_computed_map efn A' pr)
+       \<le> SPEC (\<lambda>t. less_eliminator_ref (pre_computed_map efn A' pr) t A' pl
+                    \<le> SPEC (\<lambda>c. (c , max_eliminator efn A pr) \<in> Id))"
+    unfolding max_eliminator.simps using aeq
+    by (smt (verit, best) IdI SPEC_cons_rule)
 
 qed
 
@@ -429,10 +398,10 @@ lemma max_eliminator_Id:
   assumes prel: "(pl, pr) \<in> profile_rel"
   shows "((\<lambda> A. max_eliminator_ref (pre_computed_map efn A pr) A pl),
            ((\<lambda> A.  SPEC (\<lambda> em. em = max_eliminator efn A pr))))
- \<in> \<langle>Id\<rangle>alt_set_rel \<rightarrow>  \<langle>Id\<rangle>nres_rel"
+ \<in> \<langle>Id\<rangle>finite_set_rel \<rightarrow>  \<langle>Id\<rangle>nres_rel"
 proof (rule fun_relI, rule nres_relI, rename_tac A' A)
   fix A' A :: "'a set"
-  assume arel:  "(A', A) \<in> \<langle>Id\<rangle>alt_set_rel"
+  assume arel:  "(A', A) \<in> \<langle>Id\<rangle>finite_set_rel"
   thus  "max_eliminator_ref (pre_computed_map efn A' pr) A' pl
        \<le> \<Down> Id (SPEC (\<lambda>em. em = max_eliminator efn A pr))" 
     using max_eliminator_ref_correct[THEN fun_relD, THEN nres_relD] prel set_rel_id prod_rel_id
